theories/term.v
@@ -128,50 +128,6 @@ Coercion TypI  : Typ >-> Index.
 
 (** ** Terms *)
 
-Inductive Value :=
-| NumConst  : NumType -> nat -> Value
-| Tt        : Value (* Unit value *)
-| Coderef   : nat(* module index *) -> nat (* table index *) -> list Index -> Value
-| Fold      : Value -> Value
-| Prod      : list Value -> Value
-| Ref       : Loc -> Value
-| PtrV      : Loc -> Value
-| Cap       : Value
-| Own       : Value
-| Mempack   : Loc -> Value -> Value.
-
-Inductive HeapValue :=
-| Variant : nat -> Value -> HeapValue
-| Struct  : list Value -> HeapValue
-| Array   : nat -> list Value -> HeapValue
-| Pack    : Typ -> Value ->  HeapType -> HeapValue.
-
-(* Size of a value in words. *)
-Fixpoint size_val (v : Value) : nat :=
-  match v with
-  | NumConst (Int _ i32) _ => 1
-  | NumConst (Int _ i64) _ => 2
-  | NumConst (Float f32) _ => 1
-  | NumConst (Float f64) _ => 2
-  | Tt => 1
-  | Coderef _ _ _ => 2
-  | Fold v => size_val v
-  | Prod vs => sum_list_with size_val vs
-  | Ref _ => 1
-  | PtrV _ => 1
-  | Cap => 0
-  | Own => 0
-  | Mempack _ v => size_val v
-  end.
-
-Definition size (hv : HeapValue) : nat :=
-  match hv with
-  | Variant n v => 1 + size_val v
-  | Struct vs => sum_list_with size_val vs
-  | Array i vs => sum_list_with size_val vs
-  | Pack p v ht => 1 + size_val v
-  end.
-
 Inductive IUnOp :=
 | clz | ctz | popcnt.
 
@@ -223,105 +179,60 @@ Definition ex := positive.
 (* imports *)
 Definition im := positive.
 
-Inductive basic_instr A :=
-  | Val : A -> Value -> basic_instr A
-  | Ne : A -> NumInstr -> basic_instr A
-  | Unreachable : A -> basic_instr A
-  | Nop : A -> basic_instr A
-  | Drop : A -> basic_instr A
-  | Select : A -> basic_instr A
-  | Block : A -> ArrowType -> LocalEffect -> list (basic_instr A) -> basic_instr A
-  | Loop : A -> ArrowType -> list (basic_instr A) -> basic_instr A
-  | ITE : A -> ArrowType -> LocalEffect -> list (basic_instr A) -> list (basic_instr A) -> basic_instr A
-  | Br : A -> nat -> basic_instr A
-  | Br_if : A -> nat -> basic_instr A
-  | Br_table : A -> list nat -> nat -> basic_instr A
-  | Ret : A -> basic_instr A
-  | Get_local : A -> nat -> Qual -> basic_instr A
-  | Set_local : A -> nat -> basic_instr A
-  | Tee_local : A -> nat -> basic_instr A
-  | Get_global : A -> nat -> basic_instr A
-  | Set_global : A -> nat -> basic_instr A
-  | CoderefI : A -> nat -> basic_instr A
-  | Inst : A -> list Index -> basic_instr A
-  | Call_indirect : A -> basic_instr A
-  | Call : A -> nat -> list Index -> basic_instr A
-  | RecFold : A -> Typ -> basic_instr A
-  | RecUnfold : A -> basic_instr A
-  | Group : A -> nat -> Qual -> basic_instr A
-  | Ungroup : A -> basic_instr A
-  | CapSplit : A -> basic_instr A
-  | CapJoin : A -> basic_instr A
-  | RefDemote : A -> basic_instr A
-  | MemPack : A -> Loc -> basic_instr A (* XXX Loc or not? *)
-  | MemUnpack : A -> ArrowType -> LocalEffect -> list (basic_instr A) -> basic_instr A (* binding site *)
-  | StructMalloc : A -> list Size -> Qual -> basic_instr A
-  | StructFree : A -> basic_instr A
-  | StructGet : A -> nat -> basic_instr A
-  | StructSet: A -> nat -> basic_instr A
-  | StructSwap : A -> nat -> basic_instr A
-  | VariantMalloc : A -> nat -> list Typ -> Qual -> basic_instr A
-  | VariantCase : A -> Qual -> HeapType -> ArrowType -> LocalEffect -> list (list (basic_instr A)) -> basic_instr A
-  | ArrayMalloc : A -> Qual -> basic_instr A
-  | ArrayGet : A -> basic_instr A
-  | ArraySet : A -> basic_instr A
-  | ArrayFree : A -> basic_instr A
-  | ExistPack : A -> Typ -> HeapType -> Qual -> basic_instr A
-  | ExistUnpack : A -> Qual -> HeapType -> ArrowType -> LocalEffect -> list (basic_instr A) -> basic_instr A (* binding site *)
-  | RefSplit : A -> basic_instr A
-  | RefJoin : A -> basic_instr A
-  | Qualify : A -> Qual -> basic_instr A.
+Inductive instr {A} :=
+  | INumConst (ann : A) (nt : NumType) (n : nat)
+  | IUnit (ann : A)
+  | INum (ann : A) (ni : NumInstr)
+  | IUnreachable (ann : A)
+  | INop (ann : A)
+  | IDrop (ann : A)
+  | ISelect (ann : A)
+  | IBlock (ann : A) (ta : ArrowType) (tl : LocalEffect) (es : list instr)
+  | ILoop (ann : A) (ta : ArrowType) (es : list instr)
+  | IIte (ann : A) (ta : ArrowType) (tl : LocalEffect) (es1 : list instr) (es1 : list instr)
+  | IBr (ann : A) (n : nat)
+  | IBrIf (ann : A) (n : nat)
+  | IBrTable (ann : A) (ns : list nat) (n : nat)
+  | IRet (ann : A)
+  | IGetLocal (ann : A) (n : nat) (q : Qual)
+  | ISetLocal (ann : A) (n : nat)
+  | ITeeLocal (ann : A) (n : nat)
+  | IGetGlobal (ann : A) (n : nat)
+  | ISetGlobal (ann : A) (n : nat)
+  | ICoderef (ann : A) (n : nat)
+  | IInst (ann : A) (idxs : list Index)
+  | ICallIndirect (ann : A)
+  | ICall (ann : A) (n : nat) (idxs : list Index)
+  | IRecFold (ann : A) (ty : Typ)
+  | IRecUnfold (ann : A)
+  | IGroup (ann : A) (n : nat) (q : Qual)
+  | IUngroup (ann : A)
+  | ICapSplit (ann : A)
+  | ICapJoin (ann : A)
+  | IRefDemote (ann : A)
+  | IMemPack (ann : A) (l : Loc) (* XXX Loc or not? *)
+  | IMemUnpack (ann : A) (ta : ArrowType) (tl : LocalEffect) (es : list instr)
+  | IStructMalloc (ann : A) (szs : list Size) (q : Qual)
+  | IStructFree (ann : A)
+  | IStructGet (ann : A) (n : nat)
+  | IStructSet (ann : A) (n : nat)
+  | IStructSwap (ann : A) (n : nat)
+  | IVariantMalloc (ann : A) (n : nat) (ts : list Typ) (q : Qual)
+  | IVariantCase (ann : A) (q : Qual) (th : HeapType) (ta : ArrowType) (tl : LocalEffect) (es : list (list instr))
+  | IArrayMalloc (ann : A) (q : Qual)
+  | IArrayGet (ann : A)
+  | IArraySet (ann : A)
+  | IArrayFree (ann : A)
+  | IExistPack (ann : A) (t : Typ) (th : HeapType) (q : Qual)
+  | IExistUnpack (ann : A) (q : Qual) (th : HeapType) (ta : ArrowType) (tl : LocalEffect) (es : list instr)
+  | IRefSplit (ann : A)
+  | IRefJoin (ann : A)
+  | IQualify (ann : A) (q : Qual).
 
-Arguments Val {_} _ _.
-Arguments Ne {_} _ _.
-Arguments Unreachable {_} _.
-Arguments Nop {_} _.
-Arguments Drop {_} _.
-Arguments Select {_} _.
-Arguments Block {_} _ _ _ _.
-Arguments Loop {_} _ _ _.
-Arguments ITE {_} _ _ _ _.
-Arguments Br {_} _ _.
-Arguments Br_if {_} _ _.
-Arguments Br_table {_} _ _ _.
-Arguments Ret {_} _.
-Arguments Get_local {_} _ _ _.
-Arguments Set_local {_} _ _.
-Arguments Tee_local {_} _ _.
-Arguments Get_global {_} _ _.
-Arguments Set_global {_} _ _.
-Arguments CoderefI {_} _ _.
-Arguments Inst {_} _ _.
-Arguments Call_indirect {_} _.
-Arguments Call {_} _ _ _.
-Arguments RecFold {_} _ _.
-Arguments RecUnfold {_} _.
-Arguments Group {_} _ _ _.
-Arguments Ungroup {_} _.
-Arguments CapSplit {_} _.
-Arguments CapJoin {_} _.
-Arguments RefDemote {_} _.
-Arguments MemPack {_} _ _.
-Arguments MemUnpack {_} _ _ _ _.
-Arguments StructMalloc {_} _ _ _.
-Arguments StructFree {_} _.
-Arguments StructGet {_} _ _.
-Arguments StructSet {_} _ _.
-Arguments StructSwap {_} _ _.
-Arguments VariantMalloc {_} _ _ _ _.
-Arguments VariantCase {_} _ _ _ _ _ _.
-Arguments ArrayMalloc {_} _ _.
-Arguments ArrayGet {_} _.
-Arguments ArraySet {_} _.
-Arguments ArrayFree {_} _.
-Arguments ExistPack {_} _ _ _ _.
-Arguments ExistUnpack {_} _ _ _ _ _ _.
-Arguments RefSplit {_} _.
-Arguments RefJoin {_} _.
-Arguments Qualify {_} _ _.
+Arguments instr : clear implicits.
 
 Inductive Func A :=
-  | Fun : list ex -> FunType -> list Size -> list (basic_instr A) -> Func A.
+  | Fun : list ex -> FunType -> list Size -> list (instr A) -> Func A.
 
 Arguments Fun {_} _ _ _ _.
 
@@ -330,26 +241,9 @@ Inductive Closure A :=
 
 Arguments Clo {_} _ _.
 
-Inductive admin_instr A :=
-  | Basic : basic_instr A -> admin_instr A
-  | Trap
-  | CallAdm : Closure A -> list Index -> admin_instr A
-  | Label : nat -> ArrowType -> list (admin_instr A) -> list (admin_instr A) -> admin_instr A
-  | Local : nat -> nat -> list Value -> list nat (* sizes of local slots (args + locals) *) -> list (admin_instr A) -> admin_instr A
-  | Malloc : Size -> HeapValue -> Qual -> admin_instr A
-  | Free.
-
-Arguments Basic {_} _.
-Arguments Trap {_}.
-Arguments CallAdm {_} _ _.
-Arguments Label {_} _ _ _ _.
-Arguments Local {_} _ _ _ _ _.
-Arguments Malloc {_} _ _ _.
-Arguments Free {_}.
-
 Inductive Glob A :=
-| GlobMut : Typ -> list (basic_instr A) -> Glob A
-| GlobEx : list ex -> Typ -> list (basic_instr A) -> Glob A
+| GlobMut : Typ -> list (instr A) -> Glob A
+| GlobEx : list ex -> Typ -> list (instr A) -> Glob A
 | GlobIm : list ex -> Typ -> im -> Glob A.
 
 Arguments GlobMut {_} _ _.
@@ -361,64 +255,12 @@ Definition module A :=
    list (Glob A) *
    Table)%type.
 
-Record MInst A :=
-  { func : list (Closure A);
-    glob : list (Mut * Value);
-    tab  : list (Closure A);
-  }.
-
-Arguments Build_MInst {_} _ _ _.
-
 (** Useful properties *)
-
-Lemma Value_ind' :
-  forall P : Value -> Prop,
-    (forall (n : NumType) (n0 : nat), P (NumConst n n0)) ->
-    P Tt ->
-    (forall (n n0 : nat) (l : list Index), P (Coderef n n0 l)) ->
-    (forall v : Value, P v -> P (Fold v)) ->
-    (forall l : list Value, Forall P l -> P (Prod l)) ->
-    (forall l : Loc, P (Ref l)) ->
-    (forall l : Loc, P (PtrV l)) ->
-    P Cap ->
-    P Own ->
-    (forall (l : Loc) (v : Value), P v -> P (Mempack l v)) ->
-    forall v : Value, P v.
-Proof.
-  intros P H1 H2 H3 H4 H5 H6 H7 H8 H9 H10.
-  fix IHv 1. induction v; try (now clear IHv; eauto).
-  eapply H5.
-  induction l.
-  - now constructor.
-  - constructor. eapply IHv. eassumption.
-Qed.
 
 Inductive Forall_type {A : Type} (P : A -> Type) : list A -> Type :=
 | Forall_type_nil : Forall_type P []
 | Forall_type_cons : forall (x : A) (l : list A),
     P x -> Forall_type P l -> Forall_type P (x :: l).
-
-Lemma Value_rect' :
-  forall P : Value -> Type,
-    (forall (n : NumType) (n0 : nat), P (NumConst n n0)) ->
-    P Tt ->
-    (forall (n n0 : nat) (l : list Index), P (Coderef n n0 l)) ->
-    (forall v : Value, P v -> P (Fold v)) ->
-    (forall l : list Value, Forall_type P l -> P (Prod l)) ->
-    (forall l : Loc, P (Ref l)) ->
-    (forall l : Loc, P (PtrV l)) ->
-    P Cap ->
-    P Own ->
-    (forall (l : Loc) (v : Value), P v -> P (Mempack l v)) ->
-    forall v : Value, P v.
-Proof.
-  intros P H1 H2 H3 H4 H5 H6 H7 H8 H9 H10.
-  fix IHv 1. induction v; try (now clear IHv; eauto).
-  eapply H5.
-  induction l.
-  - now constructor.
-  - constructor. eapply IHv. eassumption.
-Qed.
 
 Section TypeInd.
 
@@ -550,83 +392,3 @@ Section TypeRect.
   Qed.
   
 End TypeRect.
-
-Section InstructionInd.
-  Context
-    (A : Type)
-    (I : basic_instr A -> Prop)
-    (F : Func A -> Prop)
-    (C : Closure A -> Prop).
-
-  Context
-    (HVal : forall x v, I (Val x v))
-    (HNe : forall x ninstr, I (Ne x ninstr))
-    (HUnreachable : forall x, I (Unreachable x))
-    (HNop : forall x, I (Nop x))
-    (HDrop : forall x, I (Drop x))
-    (HSelect : forall x, I (Select x))
-    (HBlock : forall x arty leff insns, Forall I insns -> I (Block x arty leff insns))
-    (HLoop : forall x arty insns, Forall I insns -> I (Loop x arty insns))
-    (HITE : forall x arty leff insns1 insns2,
-        Forall I insns1 ->
-        Forall I insns2 ->
-        I (ITE x arty leff insns1 insns2))
-    (HBr : forall x n, I (Br x n))
-    (HBr_if : forall x n, I (Br_if x n))
-    (HBr_table : forall x ns n, I (Br_table x ns n))
-    (HRet : forall x, I (Ret x))
-    (HGet_local : forall x n qual, I (Get_local x n qual))
-    (HSet_local : forall x n, I (Set_local x n))
-    (HTee_local : forall x n, I (Tee_local x n))
-    (HGet_global : forall x n, I (Get_global x n))
-    (HSet_global : forall x n, I (Set_global x n))
-    (HCoderefI : forall x n, I (CoderefI x n))
-    (HInst : forall x ixs, I (Inst x ixs))
-    (HCall_indirect : forall x, I (Call_indirect x))
-    (HCall : forall x n ixs, I (Call x n ixs))
-    (HRecFold : forall x pt, I (RecFold x pt))
-    (HRecUnfold : forall x, I (RecUnfold x))
-    (HGroup : forall x n qual, I (Group x n qual))
-    (HUngroup : forall x, I (Ungroup x))
-    (HCapSplit : forall x, I (CapSplit x))
-    (HCapJoin : forall x, I (CapJoin x))
-    (HRefDemote  : forall x, I (RefDemote x))
-    (HMemPack   : forall x l, I (MemPack x l))
-    (HMemUnpack : forall x arty leff insns, Forall I insns -> I (MemUnpack x arty leff insns))
-    (HStructMalloc : forall x szs qual, I (StructMalloc x szs qual))
-    (HStructFree : forall x, I (StructFree x))
-    (HStructGet : forall x n, I (StructGet x n))
-    (HStructSet : forall x n, I (StructSet x n))
-    (HStructSwap : forall x n, I (StructSwap x n))
-    (HVariantMalloc : forall x n typs qual, I (VariantMalloc x n typs qual))
-    (HVariantCase : forall x qual arty leff insnss tausv,
-        Forall (Forall I) insnss ->
-        I (VariantCase x qual tausv arty leff insnss))
-    (HArrayMalloc : forall x qual, I (ArrayMalloc x qual))
-    (HArrayGet : forall x, I (ArrayGet x))
-    (HArraySet : forall x, I (ArraySet x))
-    (HArrayFree : forall x, I (ArrayFree x))
-    (HExistPack : forall x pt ht qual, I (ExistPack x pt ht qual))
-    (HExistUnpack : forall x qual arty leff insns ex , Forall I insns -> I (ExistUnpack x qual ex arty leff insns))
-    (HRefSplit : forall x, I (RefSplit x))
-    (HRefJoin : forall x, I (RefJoin x))
-    (HQualify : forall x qual, I (Qualify x qual)).
-
-  Context (HFun : forall exs fty szs insns, Forall I insns -> F (Fun exs fty szs insns)).
-
-  Context (HClo : forall n func, F func -> C (Clo n func)).
-
-  Local Ltac clear_ihs :=
-    try match goal with
-    | HI : forall x, I x, HF : forall x, F x, HC : forall x, C x |- _ => clear HI HF HC
-    end.
-
-  Local Ltac list_ind :=
-    match goal with
-    | IH : forall _, ?P _ |- Forall (Forall ?P) ?l =>
-      clear - IH; induction l; constructor; try assumption; list_ind
-    | IH : forall _, ?P _ |- Forall ?P ?l =>
-      clear - IH; induction l; constructor; auto
-    end.
-
-End InstructionInd.
